theories/LambdaWt/WtCtx.v
@@ -1,0 +1,159 @@
+Require Import Coq.Lists.List.
+Require Import ExtLib.Data.HList.
+Require Import ExtLib.Structures.Applicative.
+Require Import ChargeCore.Logics.ILogic.
+Require Import MirrorCore.LambdaWt.WtExpr.
+Require Import MirrorCore.LambdaWt.SubstWt.
+Require Import MirrorCore.LambdaWt.WtMigrator.
+
+Section simple_dep_types.
+  Variable Tsymbol : Type.
+  Variable TsymbolD : Tsymbol -> Type@{Urefl}.
+  Variable Tsymbol_eq_dec : forall a b : Tsymbol, {a = b} + {a <> b}.
+
+  Variable Esymbol : type Tsymbol -> Type.
+  Variable EsymbolD : forall t, Esymbol t -> typeD TsymbolD t.
+
+  Section with_existentials.
+    (** This is the universe with operators for [forall] and [impl] *)
+    Variable tyProp : type Tsymbol.
+    Context {LogicOps_tyProp : ILogicOps (typeD TsymbolD tyProp)}.
+    Context {Logic_tyProp : ILogic (typeD TsymbolD tyProp)}.
+
+    (** Goals **)
+    Inductive wtgoal tus tvs : Type :=
+    | wtSolved : wtgoal tus tvs
+    | wtGoal   : wtexpr Esymbol tus tvs tyProp -> wtgoal tus tvs
+    | wtConj   : wtgoal tus tvs -> wtgoal tus tvs -> wtgoal tus tvs
+    | wtHyp    : wtexpr Esymbol tus tvs tyProp -> wtgoal tus tvs -> wtgoal tus tvs
+    | wtAll    : forall t, wtgoal tus (t :: tvs) -> wtgoal tus tvs.
+    Arguments wtSolved {_ _}.
+    Arguments wtGoal {_ _} _.
+    Arguments wtConj {_ _} _ _.
+    Arguments wtHyp {_ _} _ _.
+    Arguments wtAll {_ _} _ _.
+
+    Section wtgoal_subst.
+      Context {tus tus' : list (Tuvar Tsymbol)}.
+      Variable mig : migrator Esymbol tus tus'.
+
+      Fixpoint wtgoal_subst {tvs tvs'}
+               (sVar : hlist (wtexpr Esymbol tus' tvs') tvs)
+               (gl : wtgoal tus tvs)
+      : wtgoal tus' tvs'.
+      refine
+        match gl with
+        | wtSolved => wtSolved
+        | wtGoal gl => wtGoal (subst sVar (migrate_expr mig gl))
+        | wtConj l r =>
+          wtConj (wtgoal_subst _ _ sVar l) (wtgoal_subst _ _ sVar r)
+        | wtHyp p g =>
+          wtHyp (subst sVar (migrate_expr mig p)) (wtgoal_subst _ _ sVar g)
+        | wtAll t g =>
+          wtAll t (wtgoal_subst _ _
+                                (Hcons (wtVar (Member.MZ _ _)) _) g)
+        end.
+      eapply hlist_map.
+      2: eapply sVar.
+      intros.
+      eapply (@wtexpr_lift _ _ tus' _ _ (_::nil) nil X).
+      Defined.
+    End wtgoal_subst.
+
+    Fixpoint wtgoalD {tus tvs} (g : wtgoal tus tvs) {struct g}
+    : exprT TsymbolD tus tvs (typeD TsymbolD tyProp) :=
+      match g with
+      | wtSolved => pure ltrue
+      | wtGoal g => wtexprD EsymbolD g
+      | wtConj l r =>
+        ap (ap (pure land) (wtgoalD l)) (wtgoalD r)
+      | wtHyp h g => ap (ap (pure limpl) (wtexprD EsymbolD h)) (wtgoalD g)
+      | @wtAll _ _ t g =>
+        let gD := wtgoalD g in
+        ap (T:=exprT TsymbolD tus tvs) (pure (@lforall _ _ (typeD TsymbolD t)))
+           (fun us vs v => gD us (Hcons v vs))
+      end.
+
+
+    Inductive wtctx (tus : list (Tuvar Tsymbol)) : list (type Tsymbol) -> Type :=
+    | ctx_Top : wtctx tus nil
+    | ctx_All : forall t {ts}, wtctx tus ts -> wtctx tus (t :: ts)
+    | ctx_Hyp : forall {ts}, wtexpr Esymbol tus ts tyProp ->
+                             wtctx tus ts -> wtctx tus ts
+    | ctx_Left : forall {ts}, wtgoal tus ts -> wtctx tus ts -> wtctx tus ts
+    | ctx_Right : forall {ts}, wtgoal tus ts -> wtctx tus ts -> wtctx tus ts
+(*
+    | ctx_MDelay : forall {tus' tvs},
+        migrator Esymbol tus' tus ->
+        wtctx tus' tvs -> wtctx tus tvs
+*)
+    .
+    Arguments ctx_Top {_}.
+    Arguments ctx_All {_} _ {_} _.
+    Arguments ctx_Hyp {_ _} _ _.
+    Arguments ctx_Left {_ _} _ _.
+    Arguments ctx_Right {_ _} _ _.
+(*
+    Arguments ctx_MDelay {_ _ _} _ _.
+*)
+
+    Arguments WtMigrator.vars_id {_ _ _ tvs} : rename.
+
+    Fixpoint force_ctx {tus tus' tvs} (mig : migrator Esymbol tus tus')
+             (ctx : wtctx tus tvs) : wtctx tus' tvs :=
+      match ctx in wtctx _ tvs return wtctx tus' tvs with
+      | ctx_Top => ctx_Top
+      | ctx_All t c => ctx_All t (force_ctx mig c)
+      | ctx_Hyp p c => ctx_Hyp (migrate_expr mig p) (force_ctx mig c)
+      | ctx_Left g c =>
+        ctx_Left (wtgoal_subst mig WtMigrator.vars_id g) (force_ctx mig c)
+      | ctx_Right g c =>
+        ctx_Right (wtgoal_subst mig WtMigrator.vars_id g) (force_ctx mig c)
+(*
+      | ctx_MDelay m c => force_ctx (migrator_compose m mig) c
+*)
+      end.
+
+    Fixpoint wtctxD {tus} {ts : list (type Tsymbol)} (ctx : wtctx tus ts)
+    : exprT TsymbolD tus ts (typeD TsymbolD tyProp) ->
+      exprT TsymbolD tus nil (typeD TsymbolD tyProp) :=
+      match ctx in wtctx _ ts
+            return exprT TsymbolD tus ts (typeD TsymbolD tyProp) ->
+                   exprT TsymbolD tus nil (typeD TsymbolD tyProp)
+      with
+      | ctx_Top => fun K => K
+      | ctx_All t ctx' => fun K =>
+        wtctxD ctx'
+               (fun us vs => lforall (fun v => K us (HList.Hcons v vs)))
+      | ctx_Hyp t ctx' => fun K =>
+        wtctxD ctx'
+               (fun us vs => wtexprD EsymbolD t us vs -->> K us vs)
+      | ctx_Left g ctx' => fun K =>
+        wtctxD ctx'
+               (fun us vs => wtgoalD g us vs //\\ K us vs)
+      | ctx_Right g ctx' => fun K =>
+        wtctxD ctx'
+               (fun us vs => K us vs //\\ wtgoalD g us vs)
+
+(*
+      | ctx_MDelay mig ctx' => fun K us vs =>
+        wtctxD _ _ ctx' _ _ vs
+*)
+      end.
+
+  End with_existentials.
+
+End simple_dep_types.
+
+Arguments wtgoal {_} Esymbol _ _ _.
+Arguments wtAll {_ _ _ _ _} _ _.
+Arguments wtSolved {_ _ _ _ _}.
+Arguments wtGoal {_ _ _ _ _} _.
+Arguments wtHyp {_ _ _ _ _} _ _.
+Arguments wtConj {_ _ _ _ _} _ _.
+Arguments ctx_Top {_ _ _ _}.
+Arguments ctx_All {_ _ _ _} _ {_} _.
+Arguments ctx_Hyp {_ _ _ _ _} _ _.
+Arguments ctx_Left {_ _ _ _ _} _ _.
+Arguments ctx_Right {_ _ _ _ _} _ _.
+Arguments wtgoalD {_ _ _} EsymbolD [tyProp] {_} [_ _] _ _ _.
